Inserting new material

src/dafny/Collections/Seqs.dfy
@@ -895,6 +895,27 @@ module {:options "-functionSyntax:4"} Dafny.Collections.Seq {
     forall i, j | 0 <= i < j < |a| :: lessThan(a[i], a[j])
   }
 
+  /* An element in an ordered set is called minimal, if it is less than every element of the set. */
+  ghost predicate IsMinimum<T>(R: (T, T) -> bool, m: T, s: set<T>) {
+    m in s && forall y: T | y in s :: R(m, y)
+  }
+
+  /* Any totally ordered set contains a unique minimal element. */
+  lemma LemmaUniqueMinimum<T(!new)>(R: (T, T) -> bool, s: set<T>) returns (m: T)
+    requires |s| > 0 && TotalOrdering(R)
+    ensures IsMinimum(R, m, s) && (forall n: T | IsMinimum(R, n, s) :: m == n)
+  {
+    var x :| x in s;
+    if s == {x} {
+      m := x;
+    } else {
+      var m' := LemmaUniqueMinimum(R, s - {x});
+      if
+      case R(m', x) => m := m';
+      case R(x, m') => m := x;
+    }
+  }
+
   lemma LemmaNewFirstElementStillSortedBy<T>(x: T, s: seq<T>, lessThan: (T, T) -> bool)
     requires SortedBy(s, lessThan)
     requires |s| == 0 || lessThan(x, s[0])
